rt monads: change ovalid syntax and remove oinvariant
Signed-off-by: Corey Lewis <corey.lewis@proofcraft.systems>

lib/Monads/OptionMonadWP.thy
@@ -22,13 +22,8 @@ begin
 
 (* Partial correctness. *)
 definition ovalid :: "('s \<Rightarrow> bool) \<Rightarrow> ('s \<Rightarrow> 'a option) \<Rightarrow> ('a \<Rightarrow> 's \<Rightarrow> bool) \<Rightarrow> bool"
-  ("o\<lbrace>_\<rbrace>/ _ /\<lbrace>_\<rbrace>") where
-  "o\<lbrace>P\<rbrace> f \<lbrace>Q\<rbrace> \<equiv> \<forall>s r. P s \<and> f s = Some r \<longrightarrow> Q r s"
-
-abbreviation (input)
-  oinvariant :: "('s,'a) lookup \<Rightarrow> ('s \<Rightarrow> bool) \<Rightarrow> bool" ("_ o\<lbrace>_\<rbrace>" [59,0] 60)
-where
-  "oinvariant f P \<equiv> o\<lbrace>P\<rbrace> f \<lbrace>\<lambda>_. P\<rbrace>"
+  ("\<lblot>_\<rblot>/ _ /\<lblot>_\<rblot>") where
+  "\<lblot>P\<rblot> f \<lblot>Q\<rblot> \<equiv> \<forall>s r. P s \<and> f s = Some r \<longrightarrow> Q r s"
 
 (* Total correctness. *)
 definition ovalidNF :: "('s \<Rightarrow> bool) \<Rightarrow> ('s \<Rightarrow> 'a option) \<Rightarrow> ('a \<Rightarrow> 's \<Rightarrow> bool) \<Rightarrow> bool" where
@@ -64,6 +59,10 @@ lemmas owhile_add_inv = owhile_inv_def[symmetric]
 
 
 (* WP rules for ovalid. *)
+lemma ovalid_inv[wp]:
+  "ovalid P f (\<lambda>_. P)"
+  by (simp add: ovalid_def)
+
 lemma obind_wp[wp]:
   "\<lbrakk> \<And>r. ovalid (R r) (g r) Q; ovalid P f R \<rbrakk> \<Longrightarrow> ovalid P (obind f g) Q"
   by (simp add: ovalid_def obind_def split: option.splits, fast)
